## 公式/模型
又一个大坑  
**忽略了定义**  
## 命题
(1) $\forall a,b \in R, (a+b)^2=a^2+2ab+b^2$  
(1.1) $\forall a,b,c \in R, (a+b+c)^2=a^2+b^2+c^2+2ab+2bc+2ac$   
(1.2) $\forall a_1,a_2,a_3,...,a_n \in R, (\Sigma_{i=1}^n a_i)^2=\Sigma_{i=1}^n a_i^2 + \Sigma_{j=1}^n 2 a_j a_{\[(j+1 \quad mod \quad n)+1]}$  

(2) $\forall a,b \in R, (a+b)^3=a^3+3a^2b+3ab^2+b^3$  
(2.1) $\forall a,b,c \in R, (a+b+c)^3=a^3+b^3+c^3+3a^b+3ab^2+3b^2c+3bc^2+3a^2c+3ac^2+2abc$  
(2.2)  
(2.3)  

(5) 令 $f(x)=\Sigma_{i=n}^1 a_i x^i (\forall a_i \in R)$, 且 $\exists c \in R, f(c)=0$ 则(x-c)是f(x)的因式  
> 证:
> 设f(x)除以(x-c)商为Q(x),余r.
> 则f(x)=(x-c)Q(x)+r   
> $f(c)=(c-c)Q(x)+r=r$   
> 所以若f(c)=0  
> 则 $f(x) \equiv 0 (mod \quad x-c)$
